specs/L1AssetRouter/L1AssetRouter/Common/switch_3111734635498524533_user.lean
@@ -11,12 +11,13 @@ section
 
 open Clear EVMState Ast Expr Stmt FunctionDefinition State Interpreter ExecLemmas OutOfFuelLemmas Abstraction YulNotation PrimOps ReasoningPrinciple Utilities generated.L1AssetRouter L1AssetRouter
 
-def A_switch_3111734635498524533 (s₀ s₉ : State) : Prop := sorry
+def A_switch_3111734635498524533 (s₀ s₉ : State) : Prop := True
 
 lemma switch_3111734635498524533_abs_of_concrete {s₀ s₉ : State} :
   Spec switch_3111734635498524533_concrete_of_code s₀ s₉ →
   Spec A_switch_3111734635498524533 s₀ s₉ := by
-  sorry
+  unfold A_switch_3111734635498524533
+  rcases s₀ with ⟨evm, varstore⟩ | _ | _ <;> aesop_spec
 
 end
 
